SL/VCG.thy
@@ -42,16 +42,16 @@ lemma ht_true: "ht P x UNIV"
   oops
 
 lemma hl_false [intro]: "ht {} x Q"
-  by (auto simp: ht_def seq_def test_def)
+  by (auto simp: ht_def seq_def torel_def)
 
 lemma hl_abort [hl_rules]: "ht P abort Q"
   by (auto simp: ht_def abort_def seq_def)
   
 lemma hl_skip [hl_rules]: "P \<subseteq> Q \<Longrightarrow> ht P skip Q"
-  by (auto simp: ht_def skip_def seq_def test_def)
+  by (auto simp: ht_def skip_def seq_def torel_def)
   
 lemma hl_graph [hl_rules]: "P \<subseteq> {s. case f (Some s) of None \<Rightarrow> False | Some q \<Rightarrow> q \<in> Q} \<Longrightarrow> ht P (graph f) Q"
-  apply (auto simp: ht_def graph_def seq_def test_def)
+  apply (auto simp: ht_def graph_def seq_def torel_def)
 apply (rule relcompI)
 apply auto
 by (metis (no_types, lifting) Ball_Collect case_optionE)
@@ -63,14 +63,178 @@ lemma hl_seq [hl_rules]: "ht R y Q \<Longrightarrow> ht P x R \<Longrightarrow> 
   by (force simp: ht_def seq_def)
 
 lemma hl_split: "ht P x {t. Q t} \<Longrightarrow> ht P x {t. Q' t} \<Longrightarrow> ht P x {t. Q t \<and> Q' t}"
-  by (force simp: ht_def seq_def test_def)
+  by (force simp: ht_def seq_def torel_def)
+
+definition only_modifies :: "('s \<times> 'h) option rel \<Rightarrow> ('v, 's) var \<Rightarrow> bool" where
+  "only_modifies R x \<equiv> \<forall>y s s' h h'. (<s, h>, <s', h'>) \<in> R \<longrightarrow> x \<noteq> y \<longrightarrow> val y s = val y s'"
  
+lemma tt2: "(<a>, <b>) \<in> X \<Longrightarrow> b \<in> p \<Longrightarrow> (<a>, <b>) \<in> X O \<lfloor>p\<rfloor>"
+  by (auto simp: torel_def)
+
+lemma tt2_sym: "(<a>, <b>) \<in> X O \<lfloor>p\<rfloor> \<Longrightarrow> (<a>, <b>) \<in> X \<and> b \<in> p"
+  by (auto simp: torel_def)
+
+lemma tt2': "(<a>, <b>) \<in> X \<Longrightarrow> a \<in> p \<Longrightarrow> (<a>, <b>) \<in> \<lfloor>p\<rfloor> O X"
+  by (auto simp: torel_def)
+
+lemma tt3: "(a, b) \<in> \<lfloor>P\<rfloor> \<Longrightarrow> \<exists>c. a = Some c \<and> c \<in> P \<and> a = b"
+by (auto simp: torel_def)
+
+
+record test = x :: nat
+
+lemma dd: "(<a, h ++ h'>, <aa, b>) \<in> assign (x_update, x) t \<Longrightarrow> h \<bottom> h' \<Longrightarrow> \<exists>h''. h'' \<bottom> h' \<and> h ++ h' = h'' ++ h' \<and> (<a, h>, <aa, h''>) \<in> assign (x_update, x) t"
+  by (auto simp: assign_def graph_def)
+
+lemma dd2: "(<a, h'' ++ h'>, <aa, b>) \<in> assign (x_update, x) t \<Longrightarrow> b = h'' ++ h'"
+  by (auto simp: assign_def graph_def)
+
+lemma dd3: "(<a, h'' ++ h'>, <aa, b>) \<in> assign (x_update, x) t \<Longrightarrow> aa = x_update (\<lambda>_. t a) a"
+  by (auto simp: assign_def graph_def)
+
+lemma "\<forall>e. R = subst R (x_update, x) e \<Longrightarrow> ht P (assign (x_update, x) t) Q \<Longrightarrow> ht (sep P R) (assign (x_update, x) t) (sep Q R)"
+apply (auto simp: sep_def ht_def seq_def)
+apply (drule tt3)
+apply clarsimp
+apply (case_tac z)
+apply simp
+defer
+apply clarsimp
+apply (rule tt2)
+apply clarsimp
+apply clarsimp
+apply (frule dd)
+apply clarsimp
+apply clarsimp
+apply (rule_tac x=h in exI)
+apply (rule_tac x=h' in exI)
+apply clarsimp
+apply (rule conjI)
+apply (rule dd2)
+apply assumption
+apply (rule conjI)
+prefer 2
+apply (drule dd3)
+apply clarsimp
+apply (clarsimp simp: subst_def)
+apply (erule_tac x=t in allE)
+apply force
+
+
+
+
+
+definition mod_var :: "('s \<times> 'h) option rel \<Rightarrow> ('v, 's) var set" where
+  "mod_var R \<equiv> {x. \<forall>s s' h h'. (<s, h>, <s', h'>) \<in> R \<longrightarrow> val x s \<noteq> val x s'}"
+
+
+definition var_loc :: "('s \<times> 'h) option rel \<Rightarrow> ('v, 's) var  \<Rightarrow> bool" where
+  "var_loc R x \<equiv> \<forall>s h s' h'. (<s, h>, <s', h'>) \<in> R \<longrightarrow> (\<exists>t. s' = set x (\<lambda>_. t s) s)"
+
+
+lemma "var_loc (assign (x_update, x) t) (x_update, x)"
+apply (auto simp: var_loc_def assign_def graph_def) oops
+
+lemma tt: "\<And>y z s h0 h1.
+       locality.frame op ++ op \<bottom> x \<Longrightarrow>
+       locality.safe op ++ op \<bottom> x \<Longrightarrow>
+       \<lfloor>P\<rfloor> O x \<subseteq> x O \<lfloor>Q\<rfloor> \<Longrightarrow>
+       (y, z) \<in> x \<Longrightarrow>
+       h0 \<bottom> h1 \<Longrightarrow>
+       (s, h0) \<in> P \<Longrightarrow>
+       (s, h1) \<in> R \<Longrightarrow>
+       z = fault \<Longrightarrow>
+       (<s, h0 ++ h1>, z)
+       \<in> x O \<lfloor>{(s, h ++ h') |s h h'. h \<bottom> h' \<and> (s, h) \<in> Q \<and> (s, h') \<in> R}\<rfloor>"
+sorry
+
+
+lemma tt4 [dest]: "the fault = (s, h) \<Longrightarrow> False"
+sorry
+
+lemma "\<forall>t. R = subst R v t \<Longrightarrow> var_loc x v \<Longrightarrow> frame x \<Longrightarrow> safe x \<Longrightarrow> ht P x Q \<Longrightarrow> ht (sep P R) x (sep Q R)"
+apply (auto simp: sep_def ht_def seq_def)
+apply (drule tt3)
+apply clarsimp
+apply (case_tac y)
+apply clarsimp
+apply (drule tt4)
+apply clarsimp
+apply clarsimp
+apply (rename_tac s h0 h1)
+apply (case_tac z)
+apply (clarsimp simp: tt)
+apply (case_tac a)
+apply clarsimp
+apply (rename_tac s' h)
+apply (rule tt2)
+apply clarsimp
+apply clarsimp
+apply (auto simp: frame_def)
+apply (erule_tac x=s in allE)
+apply (erule_tac x=h0 in allE)
+apply (erule_tac x=h1 in allE)
+apply (erule_tac x=s' in allE)
+apply (erule_tac x=h in allE)
+apply clarsimp
+apply (subgoal_tac "(<s, h0>, fault) \<notin> x")
+apply clarsimp
+apply (rule_tac x=ho' in exI)
+apply (rule_tac x=h1 in exI)
+apply clarsimp
+apply (subgoal_tac "(<s, h0>, <s', ho'>) \<in> \<lfloor>P\<rfloor> O x")
+prefer 2
+apply (rule tt2')
+apply clarsimp
+apply clarsimp
+apply (subgoal_tac "(<s, h0>, <s', ho'>) \<in> x O \<lfloor>Q\<rfloor>")
+prefer 2
+apply force
+apply (rule conjI)
+apply (drule tt2_sym)
+apply force
+apply (clarsimp simp: var_loc_def subst_def)
+apply (erule_tac x=s in allE)
+apply (erule_tac x=h0 in allE)
+apply (erule_tac x=s' in allE)
+apply (erule impE)
+apply (rule_tac x=ho' in exI)
+apply force
+apply clarsimp
+apply (erule_tac x=t in allE)
+apply force
+
+
+
+
+lemma "var_loc (assign v e) v \<Longrightarrow> R = subst R v (val v) \<Longrightarrow> ht P (assign v e) Q \<Longrightarrow> ht (sep P R) (assign v e) (sep Q R)"
+  apply (auto simp: sep_def ht_def seq_def)
+  apply (rule relcompI)
+  apply assumption
+  apply clarsimp
+
+declare [[show_types]]
+record testqwerty = x :: nat
+
+find_consts name: testqwerty
+lemma "var_loc (assign (x_update, x) e) (x_update, x)"
+apply (auto simp: var_loc_def assign_def graph_def)
+
+
+lemma "R = subst R v (val v) \<Longrightarrow> ht P (assign v e) Q \<Longrightarrow> ht (sep P R) (assign v e) (sep Q R)"
+  apply (auto simp: sep_def ht_def seq_def torel_def)
+  apply (rule relcompI)
+  apply assumption
+  apply clarsimp
+
+
+
 definition to_test :: "('a, 'b) pred \<Rightarrow> ('a, 'b) state set" where
   "to_test P \<equiv> {<p> | p. p \<in> P}"
 
 lemma hl_cond : "ht (b \<sqinter> P) x Q \<Longrightarrow> ht (-b \<sqinter> P) y Q \<Longrightarrow> ht P (cond (to_test b) x y) Q"
 sorry(*
-  apply (auto simp: ht_def cond_def seq_def to_test_def test_def)
+  apply (auto simp: ht_def cond_def seq_def to_torel_def torel_def)
 *)
 
 lemma hl_cond_aux [hl_rules]: "P \<subseteq> (P' \<union> - b) \<inter> (P'' \<union> b)  \<Longrightarrow> ht P' x Q \<Longrightarrow> ht P'' y Q \<Longrightarrow> ht P (cond (to_test b) x y) Q"
@@ -95,12 +259,12 @@ qed
 text {* Weakening / Strengthening / Consequence Rules *}
 
 lemma hl_pre: "P \<le> P' \<Longrightarrow> ht P' x Q \<Longrightarrow> ht P x Q"
-  by (fastforce simp: ht_def le_fun_def seq_def test_def)
+  by (fastforce simp: ht_def le_fun_def seq_def torel_def)
 
 lemma hl_post: "Q' \<le> Q \<Longrightarrow> ht P x Q' \<Longrightarrow> ht P x Q"
 sorry
 (*
-  by (fastforce simp: ht_def le_fun_def seq_def test_def)
+  by (fastforce simp: ht_def le_fun_def seq_def torel_def)
 *)
 lemma hl_classic: "P \<le> P' \<Longrightarrow> Q' \<le> Q \<Longrightarrow> ht P' x Q' \<Longrightarrow> ht P x Q"
 sorry
