HL/GCL.thy
@@ -1,0 +1,278 @@
+theory GCL
+  imports VCG "../AFP/Quantales/Quantale_Tests"
+begin
+
+(* Semantics *)
+
+primrec guards :: "('a set \<times> 'a rel) list \<Rightarrow> 'a set" ("\<G> _" [1000] 1000) where
+  "guards [] = {}"
+| "guards (x#xs) = fst x \<union> guards xs"
+
+primrec gc :: "('a set \<times> 'a rel) list \<Rightarrow> 'a rel" ("\<C> _" [1000] 1000) where
+  "gc [] = {}"
+| "gc (x#xs) = (\<lfloor>fst x\<rfloor> O (snd x)) \<union> gc xs"
+
+lemma guarded_restrictl_var [simp]: "\<lfloor>b \<union> c\<rfloor>; ((\<lfloor>b\<rfloor>;x) \<union> (\<lfloor>c\<rfloor>;y)) = (\<lfloor>b\<rfloor>;x) \<union> (\<lfloor>c\<rfloor>;y)"
+  by (force simp: seq_def)
+
+lemma guarded_restrictl: "\<lfloor>\<G> x\<rfloor>; y \<le> y"
+  by (auto simp: guards_def seq_def)
+
+lemma gc_induct [simp]: "\<lfloor>\<G> x\<rfloor>; \<C> x = \<C> x"
+  by (induct x) (force simp: seq_def)+
+
+definition alt :: "('a set \<times> 'a rel) list \<Rightarrow> 'a rel" where
+  "alt x \<equiv> (\<C> x)"
+
+lemma [simp]: "alt [(b, x), (-b, skip)] = cond b x skip"
+  by (auto simp add: alt_def cond_def skip_def seq_def)
+
+lemma [simp]: "alt [(b, x), (-b, y)] = cond b x y"
+  by (force simp add: alt_def cond_def skip_def seq_def)
+
+lemma [simp]: "alt [] = abort"
+  by (auto simp: alt_def abort_def seq_def)
+
+lemma [simp]: "alt [({}, x)] = abort"
+  by (force simp: alt_def abort_def seq_def)
+
+lemma [simp]: "alt [(UNIV, x)] = x"
+  by (auto simp: alt_def skip_def seq_def)
+
+definition repeat :: "('a set \<times> 'a rel) list \<Rightarrow> 'a rel" where
+  "repeat x \<equiv> (\<C> x)\<^sup>*;\<lfloor>-(\<G> x)\<rfloor>"
+
+lemma [simp]: "repeat [(b, x)] = cwhile b x"
+  by (simp add: repeat_def cwhile_def seq_def)
+
+lemma "repeat [(b, x), (-b, y)] = abort"
+  by (auto simp: repeat_def abort_def seq_def)
+
+lemma [simp]: "repeat [] = skip"
+  by (auto simp: repeat_def seq_def skip_def)
+
+lemma [simp]: "repeat [({}, x)] = skip"
+  by (auto simp: repeat_def seq_def skip_def)
+
+lemma [simp]: "repeat [(UNIV, x)] = abort"
+  by (auto simp: repeat_def abort_def seq_def)
+
+lemma [simp]: "repeat [(b, x), (c, y)] = cwhile (\<G> [(b, x), (c, y)]) (\<C> [(b, x), (c, y)])"
+  apply (simp add: repeat_def cwhile_def seq_def) oops
+
+lemma [simp]: "repeat [(b, x), (c, y)] = cwhile (b \<union> c) ((\<lfloor>b\<rfloor>;x) \<union> (\<lfloor>c\<rfloor>;y))"
+  apply (unfold cwhile_def)
+  apply (subst guarded_restrictl_var)
+  apply (clarsimp simp: seq_def repeat_def)
+done
+
+lemma repeat_while_eq: "repeat x = cwhile (\<G> x) (\<C> x)"
+  by (simp add: repeat_def cwhile_def)
+
+(* Hoare logic *)
+
+lemma hl_simple_alt: "ht p y q \<Longrightarrow> ht p x q \<Longrightarrow> ht p (x \<union> y) q"
+  by (force simp: ht_def seq_def)
+
+lemma hl_alt_base [hl_rules]: "ht (p \<inter> b) x q \<Longrightarrow> ht p (alt [(b, x)]) q"
+  by (auto simp: ht_def seq_def alt_def)
+
+lemma hl_alt_induct [hl_rules]: "ht (p \<inter> b) x q \<Longrightarrow> ht p (alt xs) q \<Longrightarrow> ht p (alt ((b, x) # xs)) q"
+  by (auto simp: ht_def seq_def alt_def) force+
+
+definition arepeat :: "'a set \<Rightarrow> ('a set \<times> 'a rel) list \<Rightarrow> 'a rel" where
+  "arepeat i x \<equiv> repeat x" 
+
+lemma hl_repeat: "ht ((\<G> x) \<inter> i) (\<C> x) i \<Longrightarrow> ht i (repeat x) (- (\<G> x) \<inter> i)"
+  by (auto simp: repeat_while_eq intro: hl_while)
+
+lemma hl_repeat_induct: "ht ((\<G> x) \<inter> i) (alt x) i \<Longrightarrow> ht i (repeat x) (- (\<G> x) \<inter> i)"
+  by (auto simp: alt_def intro: hl_repeat)
+
+lemma hl_arepeat:
+  "p \<subseteq> i \<Longrightarrow> - (\<G> x) \<inter> i \<subseteq> q \<Longrightarrow> ht ((\<G> x) \<inter> i) (\<C> x) i \<Longrightarrow> ht p (arepeat i x) q"
+  by (rule hl_classic) (auto simp: arepeat_def intro: hl_repeat)
+
+lemma hl_arepeat_induct [hl_rules]:
+  "p \<subseteq> i \<Longrightarrow> - (\<G> x) \<inter> i \<subseteq> q \<Longrightarrow> ht ((\<G> x) \<inter> i) (alt x) i \<Longrightarrow> ht p (arepeat i x) q"
+  by (auto simp: alt_def intro: hl_arepeat)
+
+lemma hl_gc [hl_rules]: "ht q' x q \<Longrightarrow> p \<inter> b \<subseteq> q' \<Longrightarrow> ht p (\<lfloor>b\<rfloor> O x) q"
+  by (force simp: ht_def seq_def)
+
+(* Concurrency by Non determinism *)
+
+datatype 'a lprog = Atomic nat "'a rel"
+  | Seq "'a lprog" "'a lprog"
+  | If nat "'a set" "'a lprog" "'a lprog"
+  | Loop nat "'a set" "'a lprog"
+
+primrec first :: "'a lprog \<Rightarrow> nat" where
+  "first (Atomic k a) = k"
+| "first (Seq x y) = first x"
+| "first (If k b x y) = k"
+| "first (Loop k b x) = k"
+
+primrec last :: "'a lprog \<Rightarrow> nat" where
+  "last (Atomic k a) = k"
+| "last (Seq x y) = last y"
+| "last (If k b x y) = last y"
+| "last (Loop k b x) = last x"
+
+primrec T :: "'a lprog \<Rightarrow> nat \<Rightarrow> (nat, 'a) var \<Rightarrow> ('a set \<times> 'a rel) list" where
+  "T (Atomic k R) c pc = [({s. val pc s = k}, R; assign (upd pc) (\<lambda>_. c))]"
+| "T (Seq x y) c pc = T x (first y) pc @ T y c pc"
+| "T (If k b x y) c pc = ({s. val pc s = k} \<inter> b, assign (upd pc) (\<lambda>_. first x))
+    # ({s. val pc s = k} - b, assign (upd pc) (\<lambda>_. first y))
+    # T x c pc @ T y c pc"
+| "T (Loop k b x) c pc = ({s. val pc s = k} \<inter> b, assign (upd pc) (\<lambda>_. first x))
+    # ({s. val pc s = k} - b, assign (upd pc) (\<lambda>_. c))
+    # T x k pc"
+
+
+record pc_state =
+  pcX :: nat
+  pcY :: nat
+
+definition par :: "'a pc_state_scheme lprog \<Rightarrow> 'a pc_state_scheme lprog \<Rightarrow> 'a pc_state_scheme rel" where
+  "par x y \<equiv> (assign pcX_update (\<lambda>_. 0)); (assign pcY_update (\<lambda>_. 0));
+          repeat ((T x (last x) (pcX_update, pcX) @ T y (last y) (pcX_update, pcY)))"
+
+(*
+syntax
+  "_repeat_od_inv" :: "'a set \<Rightarrow> ('a set \<times> 'a rel) list \<Rightarrow> 'a rel" ("(0inv _ //repeat// /  _ //od)" [0, 0] 61)
+
+translations
+  "inv i repeat c" == "CONST ann_repeat_od c i"
+
+
+
+record handshake_state =
+  pcX :: nat
+  pcY :: nat
+  x :: bool
+  y :: bool
+  c :: bool
+
+
+
+lemma "\<turnstile> \<lbrace> \<not> `x \<and> \<not> `y \<and> \<not> `c \<and> `pcX = 0 \<and> `pcY = 0 \<rbrace>
+    inv {s.
+      (pcX s \<le> 1 \<longrightarrow> \<not> x s) \<and>
+      (pcY s \<le> 1 \<longrightarrow> \<not> c s) \<and>
+      (pcX s \<le> 2 \<longrightarrow> \<not> y s \<or> c s) \<and>
+      (pcX s \<ge> 3 \<longrightarrow> y s \<and> c s) \<and>
+      (pcY s \<ge> 3 \<longrightarrow> x s) \<and>
+      (pcX s \<in> {0,1,2,3,4}) \<and>
+      (pcY s \<in> {0,1,2,3,4}) \<and>
+      (pcX s = 2 \<and> pcY s = 2 \<longrightarrow> x s \<or> y s) \<and>
+      (pcX s = 4 \<longrightarrow> x s) \<and>
+      (pcY s = 4 \<longrightarrow> y s \<and> c s)
+    }
+    repeat [
+      {s. pcX s = 0} \<mapsto> `y := False; `pcX := 1,
+      {s. pcX s = 1} \<mapsto> `x := True; `pcX := 2,
+      {s. pcX s = 2 \<and> y s} \<mapsto> `pcX := 3,
+      {s. pcX s = 3} \<mapsto> `x := True; `pcX := 4, 
+
+      {s. pcY s = 0} \<mapsto> `x := False; `pcY := 1,
+      {s. pcY s = 1} \<mapsto> `y := True; `c := True; `pcY := 2,
+      {s. pcY s = 2 \<and> x s} \<mapsto> `pcY := 3,
+      {s. pcY s = 3} \<mapsto> `y := True; `c := True; `pcY := 4  
+    ]
+  \<lbrace> `pcX = 4 \<and> `pcY = 4 \<and> `x \<and> `y \<and> `c \<rbrace>"
+apply (rule hoare_repeat_od_inv_tactic) 
+apply force
+apply force
+apply auto
+apply hoare
+apply force+
+done
+
+hide_const pcX pcY x y c
+
+record write_protocol =
+  w :: bool
+  r :: bool
+  f :: int
+  g :: int
+  y :: int
+  x :: int
+  pcX :: nat
+  pcY :: nat
+  c :: nat
+
+lemma "\<turnstile> \<lbrace> `w \<and> \<not>`r \<and> `f = 0 \<and> `g = 0 \<and> `y \<le> 0 \<and> `y < `x \<and> `pcX = 0 \<and> `pcY = 0 \<rbrace>
+    inv {s. 
+      (g s < f s \<or> w s) \<and> (y s \<le> f s) \<and> (g s \<le> f s) \<and>
+      (pcX s = 0 \<or> pcX s = 1) \<and>
+      (pcY s \<in> {0,1,2,3}) \<and>
+      (pcX s = 0 \<longrightarrow> y s \<le> f s) \<and>
+      (pcX s = 1 \<longrightarrow> g s < f s) \<and>
+      (pcY s = 0 \<longrightarrow> y s < x s \<or> r s) \<and>
+      (pcY s = 1 \<longrightarrow> g s < f s \<or> w s) \<and>
+      (pcY s = 2 \<longrightarrow> y s < f s \<or> w s) \<and>
+      (pcY s = 3 \<longrightarrow> y s < f s \<or> r s)
+    }
+    repeat [
+      {s. pcX s = 0 \<and> c s > 0 } \<mapsto> `f := `f + 1; `w := False; `pcX := 1,
+      {s. pcX s = 1 } \<mapsto> `g := `g + 1; `w := True; `pcX := 0; `c := `c - 1,
+
+      {s. \<not> (x s \<le> y s) \<and> pcY s = 0 } \<mapsto> `pcY := 1,
+      {s. pcY s = 1 } \<mapsto> `y := `g;  `pcY := 2,
+      {s. pcY s = 2 } \<mapsto> `r := `w; `pcY := 3,
+      {s. pcY s = 3 } \<mapsto>  `x := `f; `pcY := 0
+    ]
+  \<lbrace> `r \<and> `c = 0 \<and> `pcX = 0 \<and> `pcY = 0 \<rbrace>"
+apply (rule hoare_repeat_od_inv_tactic) 
+apply force
+apply force
+apply auto
+apply hoare
+apply force+
+done
+
+
+hide_const w r f g x y pcX pcY c
+
+record mutual_incl_protocol =
+  x :: int
+  y :: int
+  pcX :: nat
+  pcY :: nat
+  c :: bool
+
+lemma "\<turnstile> \<lbrace> `x = 0 \<and> `y = 0 \<and> `c \<and> `pcX = 0 \<and> `pcY = 0 \<and> n > 0 \<rbrace>
+    inv {s. 
+      (x s \<le> y s) \<and> (y s \<le> x s + 1) \<and>
+      (pcX s \<in> {0,1,2}) \<and>
+      (pcY s \<in> {0,1,2}) \<and>
+      (pcX s = 0 \<longrightarrow>  c s \<and> (x s = y s)) \<and>
+      (pcX s = 1 \<longrightarrow> \<not>c s \<or> (x s + 1 = y s)) \<and>
+      (pcX s = 2 \<longrightarrow> c s \<and> (x s + 1 = y s)) \<and>
+      (pcY s = 0 \<longrightarrow> c s \<or> (x s = y s)) \<and>
+      (pcY s = 1 \<longrightarrow> \<not>c s \<and> (x s = y s)) \<and>
+      (pcY s = 2 \<longrightarrow> \<not>c s \<and> (x s + 1 = y s)) \<and>
+      (\<not> c s \<and> (y s < n \<longrightarrow> c s) \<longrightarrow> pcX s = 1 \<longrightarrow> pcY s = 0 \<longrightarrow> x s \<noteq> y s)
+    }
+    repeat [
+      {s. pcX s = 0 \<and> x s < n } \<mapsto> `c := False; `pcX := 1,
+      {s. pcX s = 1 \<and> c s } \<mapsto> `pcX := 2,
+      {s. pcX s = 2 } \<mapsto> `x := `x + 1; `pcX := 0,
+
+      {s. pcY s = 0 \<and> y s < n \<and> \<not>c s } \<mapsto> `pcY := 1,
+      {s. pcY s = 1 } \<mapsto> `y := `y + 1; `pcY := 2,
+      {s. pcY s = 2 } \<mapsto> `c := True; `pcY := 0
+    ]
+  \<lbrace> `x = `y \<and> `pcX = 0 \<and> `pcY = 0 \<rbrace>"
+apply (rule hoare_repeat_od_inv_tactic) 
+apply force
+apply force
+apply auto
+apply hoare
+apply force+
+done
+
+hide_const x y pcX pcY c
+*)
+end
