HL/GCL_Examples.thy
@@ -1,0 +1,35 @@
+theory GCL_Examples
+  imports GCL_Syntax
+begin
+
+record euclids =
+  x :: nat
+  y :: nat
+
+lemma euclids: "\<turnstile> \<lbrace> `x = xo \<and> `y = yo \<rbrace>
+    inv gcd xo yo = gcd `x `y
+    do [
+      `x > `y \<rightarrow> `x := `x - `y,
+      `x < `y \<rightarrow> `y := `y - `x
+    ] od
+  \<lbrace> `x = gcd xo yo \<and> `x = `y \<rbrace>"
+  apply hoare
+  using gcd_diff1_nat gcd_nat.commute by auto
+
+hide_const x y
+
+record max =
+  x :: nat
+  y :: nat
+  z :: nat
+
+lemma max: "\<turnstile> \<lbrace> True \<rbrace>
+    if [
+      `x \<ge> `y \<rightarrow> `z := `x,
+      `y \<ge> `x \<rightarrow> `z := `y
+    ] fi
+  \<lbrace> `z = max `x `y \<rbrace>"
+  by hoare auto
+  
+hide_const x y z
+end
